Update fs_oval with spec_env. Next fs_ocomp.

seiostar/QTypes.OpenValComp.fst
@@ -6,6 +6,11 @@ open IOStar
 include QTypes.TypEnv
 include QTypes.EvalEnv
 
+module M = FStar.Monotonic.Pure
+private unfold
+let mk_pure_wp #a (wp:pure_wp' a{M.is_monotonic wp}) : pure_wp a =
+  M.intro_pure_wp_monotonicity wp; wp
+
 (** F* works better with these functions because it helps dealing with qTypes,
     even if they are synonyms *)
 
@@ -15,10 +20,48 @@ type fs_comp (t:qType) = io (fs_val t)
 type spec_env (g:typ_env) (a:qType) =
   eval_env g -> pure_wp (fs_val a)
 
-type fs_oval (g:typ_env) (t:qType) =
-  eval_env g -> fs_val t
-type fs_ocomp (g:typ_env) (t:qType) =
-  eval_env g -> fs_comp t
+let spec_env_return (#g:typ_env) (#a:qType) (x:fs_val a) : spec_env g a =
+  fun _ -> pure_return _ x
+
+let spec_env_bind (#g:typ_env) (#a:qType) (#b:qType) (wpP:spec_env g a) (wpK:(fs_val a -> spec_env g b)) : spec_env g b =
+  fun fsG -> pure_bind_wp _ _ (wpP fsG) (fun x -> wpK x fsG)
+
+let spec_env_axiom (#g:typ_env) (#a:qType) : spec_env (extend a g) a =
+  fun fsG -> pure_return _ (hd fsG)
+
+let spec_env_weaken (#g:typ_env) (#a #b:qType) (x:spec_env g a) : spec_env (extend b g) a =
+  fun fsG -> x (tail fsG)
+
+let spec_env_index (#g:typ_env) (x:var{Some? (g x)}) : spec_env g (Some?.v (g x)) =
+  fun fsG -> pure_return _ (index fsG x)
+
+val spec_env_app : #g :typ_env ->
+                #a :qType ->
+                #b :qType ->
+                wpF : spec_env g (a ^-> b) ->
+                wpX : spec_env g a ->
+                spec_env g b
+let spec_env_app #_ #a #b wpF wpX =
+  (fun fsG ->
+    pure_bind_wp _ _ (wpF fsG) (fun f' ->
+      pure_bind_wp _ _ (wpX fsG) (fun x' ->
+        pure_return _ (f' x'))))
+
+type fs_oval (g:typ_env) (t:qType) (wpG:spec_env g t) =
+  fsG:eval_env g -> PURE (fs_val t) (wpG fsG)
+
+let fs_ocomp_wp (g:typ_env) (t:qType) (wpG:spec_env g t) fsG : pure_wp (fs_comp t) =
+  // mk_pure_wp (fun (p:pure_post (fs_comp t)) -> 
+  //   forall comp. theta (comp) ⊑ wp_lift_pure_hist (wpG fsG) ==> p comp)
+  // CA: I think the previous would be intuitively what we want,
+  //     which could be simplified to the following since the operations
+  //     have no pre-conditions for now.
+  // Q:  The use of `as_requires` is weird, but we do not have a `p` to apply to `wpG`.
+  mk_pure_wp (fun (p:pure_post (fs_comp t)) -> 
+    as_requires (wpG fsG) /\ forall comp. p comp)
+
+type fs_ocomp (g:typ_env) (t:qType) (wpG:spec_env g t) =
+  fsG:eval_env g -> PURE (fs_comp t) (fs_ocomp_wp g t wpG fsG)
 
 (** Closed values **)
 let fs_val_if (#a:qType) (c:fs_val qBool) (e:fs_val a) (t:fs_val a) : fs_val a =
@@ -81,89 +124,179 @@ let fs_comp_call_val o args = io_call o args
 
 (** Open values **)
 unfold
-let fs_oval_return (g:typ_env) (#t:qType) (x:fs_val t) : fs_oval g t =
-  fun _ -> x
+let fs_oval_return (g:typ_env) (#t:qType) (x:fs_val t) 
+  : fs_oval g t (spec_env_return x)
+  = fun _ -> x
+
+open FStar.Tactics
 
 unfold
-val fs_oval_fmap : #g:typ_env ->
-                    #a:qType ->
-                    #b:qType ->
-                    p : fs_oval g a ->
-                    f : (fs_val a -> fs_val b) ->
-                    fs_oval g b
-let fs_oval_fmap p f fsG = f (p fsG)
+let fs_oval_fmap 
+  (#g:typ_env)
+  (#a:qType)
+  (#b:qType)
+  (#wpP : spec_env g a)
+  (m : fs_oval g a wpP)
+  (f : fs_val a -> fs_val b)
+  : fs_oval g b (spec_env_bind wpP (fun x -> spec_env_return (f x))) =
+  fun fsG ->
+    M.elim_pure_wp_monotonicity (wpP fsG);
+    f (m fsG)
 
 unfold
-let fs_oval_axiom (g:typ_env) (t:qType) : fs_oval (extend t g) t =
+let fs_oval_axiom (g:typ_env) (t:qType) 
+  : fs_oval (extend t g) t (spec_env_axiom) =
   fun fsG -> hd fsG
 
 unfold
-let fs_oval_weaken (#g:typ_env) (#a:qType) (b:qType) (x:fs_oval g a) : fs_oval (extend b g) a =
-  fun fsG -> x (tail fsG)
+let fs_oval_weaken (#g:typ_env) (#a:qType) (b:qType) (#wpX:spec_env g a) (x:fs_oval g a wpX) 
+  : fs_oval (extend b g) a (spec_env_weaken wpX) 
+  = fun fsG ->
+    M.elim_pure_wp_monotonicity (wpX (tail fsG));
+    x (tail fsG)
 
 unfold
-let fs_oval_var (g:typ_env) (x:var{Some? (g x)}) : fs_oval g (Some?.v (g x)) =
-  fun fsG -> index fsG x
+let fs_oval_var (g:typ_env) (x:var{Some? (g x)}) 
+  : fs_oval g (Some?.v (g x)) (spec_env_index x)
+  = fun fsG -> index fsG x
 
 unfold
 val fs_oval_app: #g : typ_env ->
                  #a : qType ->
                  #b : qType ->
-                 f :fs_oval g (a ^-> b) ->
-                 x :fs_oval g a ->
-                 fs_oval g b
-let fs_oval_app f x fsG = (f fsG) (x fsG)
+                 #wpF :spec_env g (a ^-> b) ->
+                 f :fs_oval g (a ^-> b) wpF ->
+                 #wpX : spec_env g a ->
+                 x :fs_oval g a wpX ->
+                 fs_oval g b (spec_env_app wpF wpX)
+let fs_oval_app #_ #_ #_ #wpF f #wpX x fsG = 
+  M.elim_pure_wp_monotonicity (wpF fsG);
+  M.elim_pure_wp_monotonicity (wpX fsG);
+  (f fsG) (x fsG)
+
 
 unfold
-val fs_oval_lambda : #g :typ_env ->
-                     #a :qType ->
-                     #b :qType ->
-                     body :fs_oval (extend a g) b ->
-                     fs_oval g (a ^-> b)
-let fs_oval_lambda #_ #_ body fsG x = body (stack fsG x)
+val spec_env_lambda_tot : #g :typ_env ->
+                #a :qType ->
+                #b :qType ->
+                #wpBody:spec_env (extend a g) b ->
+                body:fs_oval (extend a g) b wpBody ->
+                spec_env g (a ^-> b)
+
+let spec_env_lambda_tot #g #a #b #wpBody body fsG : pure_wp (fs_val (a ^-> b)) by (
+  norm [delta_only [`%fs_val; `%op_Hat_Subtraction_Greater; `%get_Type]]
+)= (** Cezar: this looks exactly like what F* generates **)
+  mk_pure_wp (fun (p:pure_post (fs_val (a ^-> b))) ->
+    (forall (x:a._1). auto_squash (wpBody (stack fsG x) (fun _ -> True))) /\
+    (pure_bind_wp _ _ 
+      (pure_return (fs_val (a ^-> b)) (fun x -> body (stack fsG x))))
+      (pure_return (fs_val (a ^-> b))) p)
+    // pure_return (fs_val (a ^-> b)) (fun (x:a._1) -> body (stack fsG x)) p)
+    // p (fun (x:fs_val a) -> body (stack fsG x)))
+
+unfold
+let fs_oval_lambda 
+  (#g :typ_env)
+  (#a :qType)
+  (#b :qType)
+  (#wpBody : spec_env (extend a g) b)
+  (body :fs_oval (extend a g) b wpBody)
+  : fs_oval g (a ^-> b) (spec_env_lambda_tot body) by (
+  norm [delta_only [`%fs_val; `%op_Hat_Subtraction_Greater; `%get_Type]]; (** not sure why I have to do this **)
+  simpl ())
+  = fun fsG ->
+      fun x -> body (stack fsG x)
 
 unfold
 val fs_oval_eq_string :
   #g : typ_env ->
-  s1 : fs_oval g qString ->
-  s2 : fs_oval g qString ->
-  fs_oval g qBool
-let fs_oval_eq_string s1 s2 fsG =
+  #wpS1 : spec_env g qString ->
+  s1 : fs_oval g qString wpS1 ->
+  #wpS2 : spec_env g qString ->
+  s2 : fs_oval g qString wpS2 ->
+  fs_oval g qBool (spec_env_bind wpS1 (fun s1' -> spec_env_bind wpS2 (fun s2' -> spec_env_return (s1' = s2'))))
+let fs_oval_eq_string #_ #wpS1 s1 #wpS2 s2 fsG =
+  M.elim_pure_wp_monotonicity (wpS1 fsG);
+  M.elim_pure_wp_monotonicity (wpS2 fsG);
   (s1 fsG) = (s2 fsG)
+
+val spec_env_if : #g :typ_env ->
+                #a :qType ->
+                wpC : spec_env g qBool ->
+                wpT : spec_env g a ->
+                wpE : spec_env g a ->
+                spec_env g a
+let spec_env_if #_ #a wpC wpT wpE =
+  (fun fsG ->
+    pure_bind_wp _ _ (wpC fsG) (fun r ->
+      pure_if_then_else _ r (wpT fsG) (wpE fsG)))
 
 unfold
 val fs_oval_if : #g :typ_env ->
                  #a  : qType ->
-                 c   : fs_oval g qBool ->
-                 t   : fs_oval g a ->
-                 e   : fs_oval g a ->
-                 fs_oval g a
-let fs_oval_if c t e fsG =
+                 #wpC : spec_env g qBool ->
+                 c   : fs_oval g qBool wpC ->
+                 #wpT : spec_env g a ->
+                 t   : fs_oval g a wpT ->
+                 #wpE : spec_env g a ->
+                 e   : fs_oval g a wpE ->
+                 fs_oval g a (spec_env_if wpC wpT wpE)
+let fs_oval_if #_ #_ #wpC c #wpT t #wpE e fsG =
+  M.elim_pure_wp_monotonicity (wpC fsG);
+  M.elim_pure_wp_monotonicity (wpT fsG);
+  M.elim_pure_wp_monotonicity (wpE fsG);
   if c fsG then t fsG else e fsG
 
 unfold
 val fs_oval_pair : #g : typ_env ->
                    #a : qType ->
                    #b : qType ->
-                   x : fs_oval g a ->
-                   y : fs_oval g b ->
-                   fs_oval g (a ^* b)
-let fs_oval_pair x y fsG =
+                   #wpX : spec_env g a ->
+                   x : fs_oval g a wpX ->
+                   #wpY : spec_env g b ->
+                   y : fs_oval g b wpY ->
+                   fs_oval g (a ^* b) (spec_env_bind wpX (fun x -> spec_env_bind wpY (fun y -> spec_env_return (x, y))))
+let fs_oval_pair #_ #_ #_ #wpX x #wpY y fsG =
+  M.elim_pure_wp_monotonicity (wpX fsG);
+  M.elim_pure_wp_monotonicity (wpY fsG);
   fs_val_pair (x fsG) (y fsG)
+
+val spec_env_case : #g :typ_env ->
+                #a :qType ->
+                #b  : qType ->
+                #c  : qType ->
+                wpCond : spec_env g (a ^+ b) ->
+                wpInlc : spec_env (extend a g) c ->
+                wpInrc : spec_env (extend b g) c ->
+                spec_env g c
+let spec_env_case wpCond wpInlc wpInrc =
+  (fun fsG ->
+    pure_bind_wp _ _ (wpCond fsG) (fun r ->
+      match r with
+      | Inl x -> wpInlc (stack fsG x)
+      | Inr x -> wpInrc (stack fsG x)))
 
 unfold
 val fs_oval_case : #g :typ_env ->
                   #a  : qType ->
                   #b  : qType ->
                   #c  : qType ->
-                  cond: fs_oval g (a ^+ b) ->
-                  inlc: fs_oval (extend a g) c ->
-                  inrc: fs_oval (extend b g) c ->
-                  fs_oval g c
-let fs_oval_case cond inlc inrc fsG =
+                  #wpCond : spec_env g (a ^+ b) ->
+                  cond: fs_oval g (a ^+ b) wpCond ->
+                  #wpInlc : spec_env (extend a g) c ->
+                  inlc: fs_oval (extend a g) c wpInlc ->
+                  #wpInrc : spec_env (extend b g) c ->
+                  inrc: fs_oval (extend b g) c wpInrc ->
+                  fs_oval g c (spec_env_case wpCond wpInlc wpInrc)
+let fs_oval_case #_ #_ #_ #_ #wpCond cond #wpInlc inlc #wpInrc inrc fsG =
+  M.elim_pure_wp_monotonicity (wpCond fsG);
   match cond fsG with
-  | Inl x -> inlc (stack fsG x)
-  | Inr x -> inrc (stack fsG x)
+  | Inl x -> 
+    M.elim_pure_wp_monotonicity (wpInlc (stack fsG x));
+    inlc (stack fsG x)
+  | Inr x -> 
+    M.elim_pure_wp_monotonicity (wpInrc (stack fsG x));
+    inrc (stack fsG x)
 
 (** Open computations **)
 
@@ -172,7 +305,7 @@ val fs_ocomp_return :
         g:typ_env ->
         #a:qType ->
         x:fs_comp a ->
-        fs_ocomp g a
+        fs_ocomp g a (spec_env_return x)
 let fs_ocomp_return _ x _ = x
 
 unfold
